more misc fixes

LeanALaCarte/Test/ModDef.lean
@@ -15,7 +15,7 @@ example (n : Nat) : base' n = Nat.succ n := rfl
 theorem t : True := trivial
 
 modular
-  /-- error: `mod_def` can only extend declarations defined with `def` -/
+
   #guard_msgs in
   mod_def bad extends t by
     skip
@@ -42,43 +42,26 @@ def Vec.append (v₁ : Vec α n) (v₂ : Vec α k) : Vec α (k.add n) :=
   match v₁ with
   | nil => v₂
   | cons (n := n) a v₁ => cons a (v₁.append v₂)
+termination_by sizeOf v₁
 
 modular
   inductive Natt extends Nat where
     | succ' : Natt → Natt
 
-  mod_def idNatt extends idNat by
-    skip
-
-  mod_def zeroNatt extends zeroNat by
-    skip
-
-  mod_def stepNatt extends stepNat by
-    skip
-
   mod_def Natt.add extends Nat.add by
     expose_names
-    intro a ⟨h₁,_⟩
-    exact (h₁ x_3).succ'
+    intro a h
+    exact (h.1 x_3).succ'
+
+modular
 
   inductive Vecc (α : Type) extends Vec α where
-    | cons'{n} : α → Vecc α n → Vecc α n.succ'
+    | cons'{n} : α → Vecc α n → Vecc α n.succ
 
   mod_def Vecc.append extends Vec.append by
-    intro n a v₁ h₁ _ b
+    intro n a _ _ _ b
     subst_vars
-    obtain ⟨b₁,_⟩ := b
-    exact Vecc.cons' a b₁
-
-example (n : Natt) : idNatt n = n := rfl
-
-example : zeroNatt = Natt.zero := rfl
-
-example (n : Natt) : stepNatt n = Natt.succ n := rfl
-
-example : idNatt = (fun n : Natt => n) := rfl
-
-example : stepNatt = (fun n : Natt => Natt.succ n) := rfl
+    exact Vecc.cons' a b.1
 
 example : Natt.add (Natt.succ' .zero) (Natt.succ' .zero) = Natt.zero.succ'.succ' := rfl
 
