LeanALaCarte/AuxMapping.lean
@@ -1,0 +1,25 @@
+import LeanALaCarte.Elab
+open Lean Parser Elab Meta Command
+
+def mkAuxMapping (oldName newName : Name) : TermElabM (Name × ModularExtension) := do
+  let oldInfo ← getConstInfo oldName
+  let newInfo ← getConstInfo newName
+  let oldNumArgs := oldInfo.type.getNumHeadForalls
+  let newNumArgs := newInfo.type.getNumHeadForalls
+  unless oldNumArgs <= newNumArgs do
+    throwError m!"Unexpected auxiliary mapping arity from `{oldName}` to `{newName}`\nThe new declaration has fewer arguments ({newNumArgs}) than the old one ({oldNumArgs})"
+  let numExtraArgs := newNumArgs - oldNumArgs
+  let oldArgBVar (i : Nat) : Expr := mkBVar (oldNumArgs - 1 - i)
+  let holeBVar (i : Nat) : Expr := mkBVar (oldNumArgs + (numExtraArgs - 1 - i))
+  let mut auxArgs : Array Expr := #[]
+  for i in [:oldNumArgs] do
+    auxArgs := auxArgs.push (oldArgBVar i)
+  for i in [:numExtraArgs] do
+    auxArgs := auxArgs.push (holeBVar i)
+  let auxExt : ModularExtension := {
+    translation := mkAppN (mkConst newName (oldInfo.levelParams.map .param)) auxArgs
+    levelParams := oldInfo.levelParams
+    numArgs := oldNumArgs
+    numHoles := numExtraArgs
+  }
+  return (oldName.eraseMacroScopes, auxExt)
